src/SynthesisFacts.v
@@ -1,40 +1,15 @@
 Require Import Bool List String Peano_dec.
-Require Import Common FMap Syntax Semantics SemFacts StepDet StepSeq.
+Require Import Common FMap Syntax Wf Semantics SemFacts StepDet StepSeq.
 Require Import Serial SerialFacts Simulation Predicate Synthesis.
-
-Lemma addPMsg_nil:
-  forall pmsg,
-    addPMsg pmsg nil = nil.
-Proof.
-  reflexivity.
-Qed.
-
-Lemma addPMsgs_nil:
-  forall pmsgs,
-    addPMsgs pmsgs nil = nil.
-Proof.
-  induction pmsgs; simpl; intros; auto.
-Qed.
-
-Lemma addPMsg_init:
-  forall pmsg objs,
-    getObjectStatesInit (addPMsg pmsg objs) =
-    getObjectStatesInit objs.
-Proof.
-  induction objs; simpl; intros; [reflexivity|].
-  find_if_inside; simpl; auto.
-  rewrite IHobjs.
-  reflexivity.
-Qed.
 
 Lemma addPMsgs_init:
   forall pmsgs objs,
     getObjectStatesInit (addPMsgs pmsgs objs) =
     getObjectStatesInit objs.
 Proof.
-  induction pmsgs; simpl; intros; [reflexivity|].
-  rewrite IHpmsgs.
-  apply addPMsg_init.
+  induction objs; simpl; intros; [reflexivity|].
+  rewrite IHobjs.
+  reflexivity.
 Qed.
 
 Lemma addPMsgsSys_init:
@@ -47,24 +22,14 @@ Proof.
   reflexivity.
 Qed.
 
-Lemma addPMsg_indices:
-  forall pmsg objs,
-    map (fun o => obj_idx o) (addPMsg pmsg objs) =
-    map (fun o => obj_idx o) objs.
-Proof.
-  induction objs; simpl; intros; [reflexivity|].
-  find_if_inside; simpl; auto.
-  rewrite IHobjs; reflexivity.
-Qed.
-
 Lemma addPMsgs_indices:
   forall pmsgs objs,
     map (fun o => obj_idx o) (addPMsgs pmsgs objs) =
     map (fun o => obj_idx o) objs.
 Proof.
-  induction pmsgs; simpl; intros; [reflexivity|].
-  rewrite IHpmsgs.
-  apply addPMsg_indices.
+  induction objs; simpl; intros; [reflexivity|].
+  rewrite IHobjs.
+  reflexivity.
 Qed.
 
 Lemma addPMsgsSys_indices:
@@ -80,34 +45,142 @@ Theorem simulation_pmsgs_compositional:
   forall {StateS LabelS: Type} `{HasInit StateS} `{HasLabel LabelS}
          (stepS: Step StateS LabelS)
          impl1 impl2 spec simR simP
-         (Hii: iisOf impl1 = iisOf impl2)
+         (Hidx: indicesOf impl1 = indicesOf impl2)
          (Hsim1: Simulates step_det stepS simR simP impl1 spec)
          (Hsim2: Simulates step_det stepS simR simP impl2 spec)
-         impl (Himplii: iisOf impl = iisOf impl1)
-         (Himplp: SubList (pmsgsOf impl) (pmsgsOf impl1 ++ pmsgsOf impl2)),
+         impl (Hii: indicesOf impl = indicesOf impl1)
+         (Himplp:
+            forall pmsg iobj,
+              In pmsg (obj_trs iobj) ->
+              In iobj (sys_objs impl) ->
+              exists obj,
+                obj_idx obj = obj_idx iobj /\
+                In pmsg (obj_trs obj) /\
+                In obj (sys_objs impl1 ++ sys_objs impl2)),
     Simulates step_det stepS simR simP impl spec.
 Proof.
   unfold Simulates; intros.
   specialize (Hsim1 ist1 sst1 H1 ilbl ist2).
   specialize (Hsim2 ist1 sst1 H1 ilbl ist2).
 
-  destruct ilbl.
-  - apply Hsim1.
-    eapply step_det_in_pmsgs_weakening; eauto.
-    apply iisOf_indicesOf; auto.
-  - destruct mhdl as [hdl|];
-      [|inv H2; apply Hsim1; constructor].
+  destruct ilbl as [|[hdl|]];
+    [apply Hsim1; eapply step_det_in_pmsgs_weakening; eauto|
+     |inv H2; apply Hsim1; constructor].
+  
+  match goal with
+  | [ |- ?g ] =>
+    assert (Hsp: step_det impl1 ist1 (IlblOuts (Some hdl) mouts) ist2 \/
+                 step_det impl2 ist1 (IlblOuts (Some hdl) mouts) ist2 -> g)
+      by (intro Hsp; destruct Hsp; [apply Hsim1; assumption|apply Hsim2; assumption])
+  end.
+  apply Hsp; clear Hsp Hsim1 Hsim2.
+  inv H2.
 
-    pose proof (step_det_pmsgs_in _ _ _ _ H2) as Hhdl.
-    simpl in Hhdl; destruct Hhdl as [hpmsg [? ?]].
-    specialize (Himplp _ H3).
-    apply in_app_or in Himplp.
-    destruct Himplp.
+  - specialize (Himplp _ _ H13 H5); destruct Himplp as [iobj [? [? ?]]].
+    apply in_app_or in H4; destruct H4.
+    + left.
+      replace (extOuts impl) with (extOuts impl1)
+        by (unfold extOuts, isExternal; rewrite Hii; reflexivity).
+      replace (intOuts impl) with (intOuts impl1)
+        by (unfold intOuts, isInternal; rewrite Hii; reflexivity).
+      eapply SdIntFwd; eauto.
+      unfold isInternal; rewrite <-Hii; assumption.
+    + right.
+      replace (extOuts impl) with (extOuts impl2)
+        by (unfold extOuts, isExternal; rewrite Hii, Hidx; reflexivity).
+      replace (intOuts impl) with (intOuts impl2)
+        by (unfold intOuts, isInternal; rewrite Hii, Hidx; reflexivity).
+      eapply SdIntFwd; eauto.
+      unfold isInternal; rewrite <-Hidx, <-Hii; assumption.
 
-    + apply Hsim1.
-      admit.
-    + apply Hsim2.
-      admit.
-    
-Admitted.
+  - specialize (Himplp _ _ H13 H5); destruct Himplp as [iobj [? [? ?]]].
+    apply in_app_or in H4; destruct H4.
+    + left.
+      replace (extOuts impl) with (extOuts impl1)
+        by (unfold extOuts, isExternal; rewrite Hii; reflexivity).
+      replace (intOuts impl) with (intOuts impl1)
+        by (unfold intOuts, isInternal; rewrite Hii; reflexivity).
+      eapply SdIntInit; eauto.
+      unfold isInternal; rewrite <-Hii; assumption.
+    + right.
+      replace (extOuts impl) with (extOuts impl2)
+        by (unfold extOuts, isExternal; rewrite Hii, Hidx; reflexivity).
+      replace (intOuts impl) with (intOuts impl2)
+        by (unfold intOuts, isInternal; rewrite Hii, Hidx; reflexivity).
+      eapply SdIntInit; eauto.
+      unfold isInternal; rewrite <-Hidx, <-Hii; assumption.
+Qed.
+
+Lemma buildRawSys_indicesOf:
+  forall sys, indicesOf sys = indicesOf (buildRawSys sys).
+Proof.
+  intros; destruct sys as [obs chns].
+  unfold indicesOf, buildRawSys; simpl.
+  clear chns; induction obs; [reflexivity|].
+  simpl; rewrite IHobs; reflexivity.
+Qed.
+
+Lemma addPMsgs_pmsg_in:
+  forall pmsg pmsgs obs iobj,
+    In pmsg (obj_trs iobj) ->
+    In iobj (addPMsgs pmsgs obs) ->
+    exists obj : Object,
+      obj_idx obj = obj_idx iobj /\
+      In pmsg (obj_trs obj) /\
+      In obj (obs ++ addPMsgs pmsgs (buildRawObjs obs)).
+Proof.
+  induction obs; simpl; intros; [intuition idtac|].
+  destruct H0; subst.
+  - clear IHobs.
+    unfold addPMsgsO in H; simpl in H.
+    apply in_app_or in H; destruct H.
+    + exists (addPMsgsO pmsgs
+                        {| obj_idx := obj_idx a;
+                           obj_state_init := obj_state_init a;
+                           obj_trs := nil |}); simpl; repeat split.
+      * rewrite app_nil_r; assumption.
+      * right; apply in_or_app; right.
+        left; reflexivity.
+    + exists a; repeat split; auto.
+  - specialize (IHobs _ H H0).
+    destruct IHobs as [obj [? [? ?]]].
+    exists obj; repeat split; auto.
+    right.
+    apply in_or_app.
+    apply in_app_or in H3; destruct H3.
+    + left; assumption.
+    + right; right; auto.
+Qed.
+
+Lemma addPMsgsSys_pmsg_in:
+  forall sys pmsgs pmsg iobj,
+    In pmsg (obj_trs iobj) ->
+    In iobj (sys_objs (addPMsgsSys pmsgs sys)) ->
+    exists obj : Object,
+      obj_idx obj = obj_idx iobj /\
+      In pmsg (obj_trs obj) /\
+      In obj (sys_objs sys ++ sys_objs (addPMsgsSys pmsgs (buildRawSys sys))).
+Proof.
+  intros; destruct sys as [obs chns]; simpl in *.
+  apply addPMsgs_pmsg_in; auto.
+Qed.
+
+Corollary simulation_pmsgs_added:
+  forall {StateS LabelS: Type} `{HasInit StateS} `{HasLabel LabelS}
+         (stepS: Step StateS LabelS)
+         impl pmsgs spec simR simP
+         (Hsim1: Simulates step_det stepS simR simP impl spec)
+         (Hsim2: Simulates step_det stepS simR simP
+                           (addPMsgsSys pmsgs (buildRawSys impl)) spec),
+    Simulates step_det stepS simR simP (addPMsgsSys pmsgs impl) spec.
+Proof.
+  intros.
+  eapply simulation_pmsgs_compositional
+    with (impl1:= impl) (impl2:= addPMsgsSys pmsgs (buildRawSys impl)); eauto.
+  - rewrite addPMsgsSys_indices.
+    apply buildRawSys_indicesOf.
+  - apply addPMsgsSys_indices.
+  - clear; intros.
+    apply addPMsgsSys_pmsg_in; auto.
+Qed.
 
